Partial class type parameter variance checking

Source/Dafny/Resolver.cs
@@ -3449,6 +3449,14 @@ namespace Microsoft.Dafny {
         foreach (TopLevelDecl d in declarations) {
           if (d is IteratorDecl || d is ClassDecl) {
             // TODO: option to opt-in to this
+            var dd = (ClassDecl)d;
+            foreach(var member in dd.Members) {
+              // TODO: other cases
+              if (member is Method method) {
+                method.Ins.Iter(formal => CheckVariance(formal.Type, method, TypeParameter.TPVariance.Contra, false));
+                method.Outs.Iter(formal => CheckVariance(formal.Type, method, TypeParameter.TPVariance.Co, false));
+              }
+            }
             // foreach (var tp in d.TypeArgs) {
             //   if (tp.Variance != TypeParameter.TPVariance.Non) {
             //     reporter.Error(MessageSource.Resolver, tp.tok, "{0} declarations only support non-variant type parameters", d.WhatKind);
